wip: start work on SKI basis

Rz/Algebra/PCA.lean
@@ -42,12 +42,24 @@ macro_rules
 class PAS (α : Type u) extends HasEval α where
   /-- The evaluation relation is functional. -/
   eval_functional : (ρ : Bwd α) → (e : FreeMagma α) → (a a' : α) → ρ ⊢ e ⇓ a → (ρ ⊢ e ⇓ a') → a = a'
-  eval_var : (ρ : Bwd α) → (x : Fin ρ.length) → ρ ⊢ $(FreeMagma.var x) ⇓ ρ.get x
-  eval_oob : (ρ : Bwd α) → (x : Nat) → ρ.length ≤ x → ρ ⊢ $(FreeMagma.var x) ↑
-  eval_const : (ρ : Bwd α) → (a : α) → ρ ⊢ a ⇓ a
-  eval_ap : (ρ : Bwd α) → (e₁ e₂ : FreeMagma α) → (a₁ a₂ : α) → ρ ⊢ e₁ ⇓ a₁ → ρ ⊢ e₂ ⇓ a₂ → ρ ⊢ e₁ e₂ ≃ a₁ a₂
+  var_eval : (ρ : Bwd α) → (x : Fin ρ.length) → ρ ⊢ $(FreeMagma.var x) ⇓ ρ.get x
+  var_oob : (ρ : Bwd α) → (x : Nat) → ρ.length ≤ x → ρ ⊢ $(FreeMagma.var x) ↑
+  const_eval : (ρ : Bwd α) → (a : α) → ρ ⊢ a ⇓ a
+  ap_eval : {ρ : Bwd α} → {e₁ e₂ : FreeMagma α} → {a₁ a₂ : α} → ρ ⊢ e₁ ⇓ a₁ → ρ ⊢ e₂ ⇓ a₂ → ρ ⊢ e₁ e₂ ≃ a₁ a₂
+  ap_left_defined : {ρ : Bwd α} → {e₁ e₂ : FreeMagma α} → ρ ⊢ e₁ e₂ ↓ → ρ ⊢ e₁ ↓
+  ap_right_defined : {ρ : Bwd α} → {e₁ e₂ : FreeMagma α} → ρ ⊢ e₁ e₂ ↓ → ρ ⊢ e₂ ↓
 
+theorem PAS.const_defined [PAS α] (ρ : Bwd α) (a : α) : ρ ⊢ a ↓ :=
+  ⟨ a , PAS.const_eval ρ a ⟩
 
+theorem PAS.ap_defined
+  [PAS α]
+  {ρ : Bwd α} {e₁ e₂ : FreeMagma α} {a₁ a₂ : α}
+  (e₁_def : ρ ⊢ e₁ ⇓ a₁) (e₂_def : ρ ⊢ e₂ ⇓ a₂)
+  (v_def : ρ ⊢ a₁ a₂ ↓)
+  : ρ ⊢ e₁ e₂ ↓ :=
+    let ⟨ w , h ⟩ := v_def
+    ⟨ w , (ap_eval e₁_def e₂_def).2 w h ⟩
 
 /-- Partial Combinatory Algebras. -/
 class PCA (α : Type u) extends PAS α where
@@ -58,13 +70,103 @@ class PCA (α : Type u) extends PAS α where
   /-- Bracket abstraction has a β-law. -/
   abs_eval : (ρ : Bwd α) → (a : α) → (e : FreeMagma α) → ρ ⊢ $(abs e) a ≃ $(e [ a ])
 
+/-!
+# SKI forms a basis for PCAs (and v.v.)
+-/
 
 class SKI (α : Type u) extends PAS α where
   s : α
   k : α
   i : α
-  s_defined : (a b : α) → .nil ⊢ s a b ↓
-  k_defined : (a : α) → .nil ⊢ k a ↓
-  s_eval : (a b c : α) → .nil ⊢ s a b c ≃ ((a b) (a c))
-  k_eval : (a b : α) → .nil ⊢ k a b ⇓ a
-  i_eval : (a : α) → .nil ⊢ i a ⇓ a
+  s_defined_2 : {ρ : Bwd α} → {e₁ e₂ : FreeMagma α} → ρ ⊢ e₁ ↓ → ρ ⊢ e₂ ↓ → ρ ⊢ s e₁ e₂ ↓
+  k_defined_const : (ρ : Bwd α) → (a : α) → ρ ⊢ k a ↓
+  s_eval_const : (ρ : Bwd α) → (a b c : α) → ρ ⊢ s a b c ≃ (a b) (a c)
+  k_eval_const : (ρ : Bwd α) → (a b : α) → ρ ⊢ k a b ⇓ a
+  i_eval_const : (ρ : Bwd α) → (a : α) → ρ ⊢ i a ⇓ a
+
+namespace SKI
+
+open SKI
+
+
+theorem s_defined_1
+  [A : SKI α]
+  {ρ : Bwd α} {e : FreeMagma α}
+  (e_defined : ρ ⊢ e ↓)
+  : ρ ⊢ A.s e ↓ :=
+  PAS.ap_left_defined (s_defined_2 e_defined (PAS.const_defined ρ k))
+  -- have ⟨ a , a_eval ⟩ := e_defined
+  -- apply PAS.ap_defined
+  -- · apply PAS.const_eval
+  -- · exact a_eval
+  -- · apply s_defined_1_const
+
+-- theorem s_defined_2
+--   [A : SKI α]
+--   {ρ : Bwd α} {e₁ e₂ : FreeMagma α}
+--   (e₁_defined : ρ ⊢ e₁ ↓) (e₂_defined : ρ ⊢ e₂ ↓)
+--   : ρ ⊢ A.s e₁ e₂ ↓ :=
+--   have ⟨ a₁ , a₁_eval ⟩ := e₁_defined
+--   have ⟨ a₂ , a₂_eval ⟩ := e₂_defined
+--   have ⟨ a₃ , a₃_eval ⟩ := s_defined_2_const ρ a₁ a₂
+--   have cool := (PAS.ap_eval _ _)
+--   -- ⟨ a₃ , (PAS.ap_eval ((PAS.ap_eval (PAS.const_eval ρ A.s) a₁_eval).2 _ _) a₂_eval).2 a₃ _ ⟩
+--   -- have ⟨ a₁ , a₁_eval ⟩ := e₁_defined
+--   -- have ⟨ a₂ , a₂_eval ⟩ := e₂_defined
+--   -- apply PAS.ap_defined
+--   -- · sorry
+--   -- · sorry
+--   -- · sorry
+--   -- PAS.ap_defined a₁_eval a₂_eval _
+--   -- apply PAS.ap_defined
+--   -- · exact a₁_eval
+--   -- · sorry
+--   -- · sorry
+
+
+@[simp] def abs [SKI α] : FreeMagma α → FreeMagma α
+| .var 0 => .const i
+| .var (n+1) => .ap (.const k) (.var n)
+| .const a => .ap (.const k) (.const a)
+| .ap e₁ e₂ => .ap (.ap (.const s) (abs e₁)) (abs e₂)
+
+def abs_defined [SKI α] (ρ : Bwd α) (e : FreeMagma α) (h : e.fv ≤ ρ.length + 1) : ρ ⊢ $(SKI.abs e) ↓ := by
+  match e with
+  | .var 0 => simp; apply PAS.const_defined
+  | .var (n+1) =>
+    simp
+    apply PAS.ap_defined
+    · apply PAS.const_eval
+    · apply PAS.var_eval ρ ⟨ n , Nat.le_of_succ_le_succ h ⟩
+    · apply SKI.k_defined_const
+  | .const a =>
+    simp
+    apply PAS.ap_defined
+    · apply PAS.const_eval
+    · apply PAS.const_eval
+    · apply SKI.k_defined_const
+  | .ap e₁ e₂ =>
+    simp
+    apply s_defined_2
+    · have : e₁.fv ≤ ρ.length + 1 := Trans.trans (FreeMagma.fv_left_le_fv_ap e₁ e₂) h
+      exact SKI.abs_defined ρ e₁ this
+    · have : e₂.fv ≤ ρ.length + 1 := Trans.trans (FreeMagma.fv_right_le_fv_ap e₁ e₂) h
+      exact SKI.abs_defined ρ e₂ this
+
+end SKI
+    -- exists _
+    -- sorry
+    -- exact ⟨ _ , _ ⟩
+    -- -- have ⟨  ⟩
+    -- sorry
+    -- -- apply PAS.ap_defined
+    -- -- · sorry
+    -- -- · exact a₂_defined
+    -- -- · sorry
+    -- -- -- · apply PAS.ap_defined
+    -- -- --   · apply PAS.const_eval
+    -- -- --   · apply PAS.const_eval
+    -- -- --   · apply PAS.ap_defined
+    -- -- --     · sorry
+    -- -- --     · sorry
+    -- -- --     · sorry
